more on graph model

coq/graph_model.v
@@ -1,17 +1,28 @@
-Require Export lc.tactics.
 Require Import Coq.Logic.FunctionalExtensionality.
-Require Import lc.SetsAsPredicates.
+Require Import Coq.Classes.RelationClasses.
+Require Coq.Relations.Relation_Definitions.
+Require Import Lia.
 
-Require Import lc.env.
+Require Export lc.tactics.
+Require Import lc.SetsAsPredicates.
+Require Import lc.AssocList.
+
 
 (* https://github.com/jsiek/denotational_semantics/blob/master/agda/PValueCBV.agda *)
 
+(* Λ  \Lambda
+   ▩  \squarecrossfill 
+   ↦  \mapsto  
+   ⤇ \Mapsto  
+   ●  \CIRCLE 
+   ⊆  \subseteq   (Included)
+*)
 
 
 Inductive Value : Type :=
   | v_nat : nat -> Value 
   | v_map : list Value -> Value -> Value
-    (* trivial function value, evaluated but never applied *)
+    (* trivial function value, evaluated to a value but never applied *)
   | v_fun : Value
 .
 
@@ -93,7 +104,7 @@ Qed.
 (*  Abstraction followed by Application is the identity ------------------- *)
 
 Definition continuous (F : P Value -> P Value) : Set :=
-  forall X E, mem E ⊆ F X -> nonempty X 
+  forall X E, mem E ⊆ F X -> nonemptyT X 
          -> exists D, (mem D ⊆ X) /\ ((mem E) ⊆ F (mem D)) /\ D <> nil.
 
 Definition monotone (F : P Value -> P Value) : Set := 
@@ -101,7 +112,7 @@ Definition monotone (F : P Value -> P Value) : Set :=
 
 (* Λ-▪-id *)
 Lemma Λ_APPLY_id { F X } :
-  continuous F -> monotone F -> nonempty X 
+  continuous F -> monotone F -> nonemptyT X 
   -> (Λ F) ▩ X ≃ F X.
 Proof. 
   intros Fcont Fmono NEX.
@@ -126,83 +137,136 @@ Qed.
 
 Definition Env := GEnv (P Value).
 
-Definition ne (s : P Value) : Type := { x : Value & s x }.
-
-Definition nonempty_env (ρ : Env) : Type := forall x, ne (ρ x).
-
-(* Definition nonempty_env : Env -> Prop := fun ρ => forall x, Inhabited  _ (ρ x). *)
-
-Definition sub_env ( ρ1 : Env ) (ρ2: Env) : Prop :=
-  forall x, ρ1 x ⊆ ρ2 x.
-
-Infix "⊆e" := sub_env (at level 50).
-
-#[global] Instance Transitive_sub_env : Transitive sub_env.
-Proof. 
-  unfold Transitive. intros x y z S1 S2.
-  intros w. specialize (S1 w). specialize (S2 w).
-  transitivity (y w); auto.
-Qed.
-
+Module EnvNotations.
+Notation "ρ ⋅ x" := (access (fun _ => False) ρ x) (at level 50).
+Infix "⊔e" := (map2 Union) (at level 60).
+Infix "⊆e" := (all2 Included) (at level 50).
+End EnvNotations.
 Import EnvNotations.
 
-Lemma extend_nonempty_env {ρ x X} : 
-  nonempty_env ρ -> ne X -> nonempty_env (x ⤇ X ● ρ).
-Proof.                                                
-  intros NEP NEX.
-  intro y. unfold env_cons.
-  destruct (x == y); eauto.
+(* This cannot be part of the Env module because we need to know the type
+   of the domain *)
+Ltac gather_atoms ::=
+  let A := gather_atoms_with (fun x : vars => x) in
+  let B := gather_atoms_with (fun x : var => {{ x }}) in
+  let C := gather_atoms_with (fun x => fv_tm x) in
+  let D := gather_atoms_with (fun x : list (atom * P Value) => dom x) in
+  constr:(A \u B \u C \u D).
+
+(* ---------------------------------------------------- *)
+
+(* Sub environments *)
+
+Definition sub_env : Env -> Env -> Prop := all2 Included.
+
+Lemma all2_refl {F : P Value -> P Value -> Prop} `{Reflexive _ F} {ρ} : uniq ρ -> all2 F ρ ρ.
+Proof. induction 1; eauto. Qed.
+
+Hint Resolve all2_refl.
+
+Lemma Reflexive_sub_env {ρ:Env} : uniq ρ -> ρ ⊆e ρ.
+Proof.
+  intros. eapply all2_refl; auto.
 Qed.
 
-Lemma env_ext {ρ ρ' y X} :
-  ρ ⊆e ρ' -> forall x , (y ⤇ X ● ρ) x ⊆ (y ⤇ X ● ρ' ) x.
-Proof. 
-  intros. unfold env_cons.
-  destruct (y == x); eauto. reflexivity.
-Qed.
+#[export] Hint Resolve Reflexive_sub_env : core.
 
-(* A finite environemtn has a list of values for 
+#[export] Instance Transitive_sub_env : Transitive sub_env.
+Proof. typeclasses eauto. Qed.
+
+Lemma extend_sub_env {ρ ρ':Env}{y X} :
+  y `notin` dom ρ ->
+  ρ ⊆e ρ' -> (y ~ X ++ ρ) ⊆e (y ~ X ++ ρ' ).
+Proof. intros; econstructor; eauto. reflexivity. Qed.
+
+(* ---------------------------------------------------- *)
+
+(* Nonempty environments *)
+
+Definition ne (s : P Value) : Type := { x : Value & x ∈ s }.
+
+Definition nonempty_env : Env -> Type := allT ne.
+
+(* A finite environment has a list of values for 
    each variable. *)
-Definition finite_env (ρ : Env) : Prop :=
-  forall x , exists E , (ρ x ≃ mem E) /\ E <> nil.
+Definition finite (X : P Value) : Prop := exists E, (X ≃ mem E) /\ E <> nil.
+Definition finite_env : Env -> Type := allT finite.
 
-Definition env_union (ρ1 ρ2 : Env) : Env := 
-  fun x v => ρ1 x v \/ ρ2 x v.
 
-Infix "⊔e" := env_union (at level 60).
+Lemma extend_nonempty_env {ρ x X} : 
+  x `notin` dom ρ ->
+  ne X -> 
+  nonempty_env ρ -> nonempty_env (x ~ X ++ ρ).
+Proof. intros Fr NEP NEX. eapply allT_cons; eauto. Qed.
+
+(* ----------------------------------------------------- *)
+
+(* Join environments *)
 
 Lemma join_finite_env {ρ1 ρ2} : 
-  finite_env ρ1
+  same_scope ρ1 ρ2 
+  -> finite_env ρ1
   -> finite_env ρ2
   -> finite_env (ρ1 ⊔e ρ2).
-Proof. 
-  intros f1 f2 x.
-  move: (f1 x) => [E1 [ pE1 NE1 ]]. 
-  move: (f2 x) => [E2 [ pE2 NE2 ]].
-  exists (E1 ++ E2).
-  repeat split.
-  intros v [ p1x | p2x ].
-Admitted.
+Proof.
+  move: ρ2.
+  induction ρ1 as [|[x1 v1] r1].
+  all: intros ρ2 sc h1; destruct ρ2 as [|[x2 v2] r2]; intros h2; simpl; eauto.
+  inversion h1; subst; clear h1.
+  inversion h2; subst; clear h2.
+  destruct (x1 == x2); subst.
+  + econstructor; eauto. eapply IHr1; eauto. inversion sc. auto.
+    rewrite sub_dom1; auto.
+    destruct H3 as [E1 [s1 u1]].
+    destruct H5 as [E2 [s2 u2]].
+    exists (E1 ++ E2).
+    split.
+    rewrite -> s1.
+    rewrite -> s2.
+    rewrite union_mem. reflexivity.
+    intro h.
+    apply u2. 
+    destruct E1. simpl in h. auto.
+    done.
+  + assert False. inversion sc. subst. done. done.
+Qed.
 
-Lemma join_lub {ρ ρ1 ρ2} :
+Lemma join_lub {ρ ρ1 :Env} :
+  same_scope ρ1 ρ ->
+  forall ρ2, same_scope ρ2 ρ ->
   ρ1 ⊆e ρ -> ρ2 ⊆e ρ -> (ρ1 ⊔e ρ2) ⊆e ρ.
 Proof.
-  intros p1p p2p x v [vp1x | vp2x].
-  eapply p1p; eauto.
-  eapply p2p; eauto.
+  intro SS1.
+  induction SS1; intros ρ2 SS2; inversion SS2; subst.
+  simpl. auto.
+  intros.
+  simpl.
+  inversion H1. inversion H2. subst.
+  rewrite eq_dec_refl.
+  eapply all2_cons; eauto.
+  rewrite sub_dom1. auto.
+  rewrite -> H21.
+  rewrite -> H13.
+  rewrite union_idem.
+  reflexivity.
 Qed.
+  
 
-Lemma join_sub_left {ρ1 ρ2} : 
+Lemma join_sub_left {ρ1 ρ2 : Env} : 
+  same_scope ρ1 ρ2 ->
   ρ1 ⊆e (ρ1 ⊔e ρ2).
 Proof.
-  intros x d z. left. eauto.
-Qed.
+  intros h.
+  induction h; simpl.
+Admitted.
 
-Lemma join_sub_right {ρ1 ρ2} : 
+Lemma join_sub_right {ρ1 ρ2 : Env} : 
+  same_scope ρ1 ρ2 ->
   ρ2 ⊆e (ρ1 ⊔e ρ2).
 Proof.
-  intros x d z. right. eauto.
-Qed.
+Admitted.
+
+(* --- Monotone --------------- *)
 
 Definition monotone_env (D : Env -> P Value) := 
  forall ρ ρ' , ρ ⊆e ρ' -> (D ρ) ⊆ D ρ'.
@@ -218,17 +282,26 @@ Definition monotone_env (D : Env -> P Value) :=
 (* Continuous ----------------------------------------- *)
 
 Definition continuous_In (D:Env -> P Value) (ρ:Env) (v:Value) : Prop :=
-  v ∈ D ρ -> exists ρ' , finite_env ρ' /\ ρ' ⊆e ρ /\ (v ∈ D ρ').
+  v ∈ D ρ -> exists ρ' , exists (pf : finite_env ρ'),  ρ' ⊆e ρ /\ (v ∈ D ρ').
 
 Definition continuous_env (D:Env -> P Value) (ρ:Env) : Prop :=
   forall v, continuous_In D ρ v.
 
 (* creates an environment that maps each variable x to a singleton 
    set of some element in ρ x *)
-Definition initial_finite_env (ρ : Env) (NE : nonempty_env ρ) : Env :=
-  fun x => match (NE x) with 
-        | existT _ y _ => ⌈ y ⌉
-        end.
+Definition initial_finite_env (ρ : Env) (NE : nonempty_env ρ) : Env.
+  induction NE. exact nil.
+  destruct f as [V v].
+  exact (cons (x, ⌈ V ⌉) IHNE).
+Defined.
+
+Lemma initial_finite_dom : forall E NE, dom (initial_finite_env E NE) = dom E.
+Proof.
+  induction NE; simpl. auto.
+  destruct f as [v w]. simpl. congruence.
+Qed. 
+
+Hint Rewrite initial_finite_dom : rewr_list.
 
 Lemma singleton_mem : forall v : Value,  ⌈ v ⌉ ⊆ mem (v :: nil).
 Proof. intro v. econstructor. inversion H. done. Qed.
@@ -238,75 +311,101 @@ Proof. intro v. cbv. intros. inversion H. subst. econstructor; eauto. done. Qed.
 
 #[global] Hint Resolve singleton_mem mem_singleton : core. 
 
+Lemma finite_singleton : forall v, finite ⌈ v ⌉.
+Proof. intro v. unfold finite. exists (cons v nil).
+       split. split. eauto. eauto. done.
+Qed.
+
+#[global] Hint Resolve finite_singleton : core. 
+
+
 Lemma initial_fin (ρ : Env) (NE : nonempty_env ρ) :
   finite_env (initial_finite_env ρ NE).
 Proof.
-  intros x.
-  unfold initial_finite_env.
-  unfold nonempty_env in NE.
-  move: (NE x) => [ v w ].
-  exists (cons v nil).
-  repeat split.
-  + eauto. 
-  + eauto.
-  + done.
+  induction NE.
+  simpl. econstructor.
+  simpl. destruct f as [v w].
+  econstructor; eauto.
+  rewrite initial_finite_dom. auto.
 Qed.
 
+#[global] Hint Resolve initial_fin : core. 
 
 
 Lemma initial_fin_sub (ρ : Env) (NE : nonempty_env ρ) :
   initial_finite_env ρ NE ⊆e ρ.
 Proof.
-  intros x y vinit.
-  unfold initial_finite_env in *.
-  unfold nonempty_env in NE.
-  destruct (NE x) as [v wpx].
-  inversion vinit. subst. auto.
+  induction NE; simpl. econstructor.
+  destruct f as [v wpx].
+  econstructor. auto.
+  rewrite initial_finite_dom. auto.
+  intros z y. inversion y. subst. unfold In. auto.
 Qed.
+
+#[global] Hint Resolve initial_fin_sub : core. 
+
 
 (* single-env maps x to D and any other variable y to something in ρ y. *)
-Definition single_env (x : atom) (D : P Value) (ρ : Env) (NE : nonempty_env ρ) : Env :=
-  fun y => match (x == y) with
-        | left _ => D
-        | right _ => let (v,_) := (NE y) in  ⌈ v ⌉
-        end.
+Definition single_env (x : atom) (D : P Value) (ρ : Env) 
+  (NE : nonempty_env ρ) : Env :=
+  update x D (initial_finite_env ρ NE).
 
+  
 Lemma single_fin { v x ρ NE } : 
   finite_env (single_env x ⌈ v ⌉ ρ NE).
-Proof.        
-  intros y. 
-  unfold single_env.
-  unfold nonempty_env in NE.
-  destruct (x == y).
-  + subst. exists (cons v nil).
-    repeat split; eauto. done.
-  + move: (NE y) => [ w _ ].
-    exists (cons w nil).
-    repeat split; eauto. done.
-Qed.
+Proof.
+  induction NE; unfold finite_env; eauto.
+  unfold single_env; econstructor.
+  unfold single_env. simpl. destruct f.
+  destruct (x == x0) eqn:EQ.
+  + subst. rewrite update_eq_var. 
+    econstructor.
+    eapply initial_fin. simpl_env. auto. auto.
+  + rewrite update_neq_var; eauto. econstructor; eauto. simpl_env. auto.
+Qed.    
+
+#[global] Hint Resolve single_fin : core. 
+
 
 Lemma single_sub { ρ x v } :
   forall (NE : nonempty_env ρ),
-    v ∈ ρ x 
+    v ∈ ρ ⋅ x 
   -> (single_env x ⌈ v ⌉ ρ NE) ⊆e ρ.
 Proof.
-  intros NE vpx y w sing.
-  unfold single_env in sing.
-  destruct (x == y).
-  + inversion sing. subst.
-    auto.
-  + destruct (NE y) as [u epy].
-    inversion sing. subst.
-    auto.
+  intros NE.
+  induction NE.
+  all: intros vpe. inversion vpe.
+  unfold single_env.
+  simpl. destruct f. simpl.
+  simpl in vpe.
+  destruct (x == x0).
+  + subst. econstructor; eauto.
+    simpl_env. auto.
+    intros x h. inversion h. subst. auto.
+  + econstructor; eauto. 
+    simpl_env. auto.
+    intros y h. inversion h. subst. unfold In. auto.
 Qed.
+
+#[global] Hint Resolve single_sub : core. 
+
 
 (* v∈single[xv]x  *)
 Lemma v_single_xvx {v x ρ NE} : 
-  v ∈ single_env x ⌈ v ⌉ ρ NE x.
+  x `in` dom ρ ->
+  v ∈ (single_env x ⌈ v ⌉ ρ NE ⋅ x).
 Proof.
   unfold single_env.
-  destruct (x == x). reflexivity. done.
+  move: NE.
+  induction NE; intro h. fsetdec.
+  simpl. destruct f. simpl.
+  destruct (x == x0) eqn:EQ. subst. simpl.
+  rewrite eq_dec_refl. econstructor; eauto.
+  simpl. rewrite EQ. simpl in h. eapply IHNE; auto. fsetdec.
 Qed.  
+
+#[global] Hint Resolve v_single_xvx : core. 
+
 
 
 (* continuous-∈⇒⊆ *)
@@ -314,7 +413,7 @@ Lemma continuous_In_sub E ρ (NE : nonempty_env ρ) :
    monotone_env E
    -> forall V, mem V ⊆ E ρ
    -> (forall v, v ∈ mem V -> continuous_In E ρ v)
-   -> exists ρ', finite_env ρ' /\ ρ' ⊆e ρ /\ (mem V ⊆ E ρ').
+   -> exists ρ', exists (pf : finite_env ρ') ,  ρ' ⊆e ρ /\ (mem V ⊆ E ρ').
 Proof.
   intros me V VE vcont.
   induction V.
@@ -330,13 +429,17 @@ Proof.
     econstructor; eauto.
     eapply VE. econstructor; eauto.
     exists (ρ1 ⊔e ρ2).
+    have S1: same_scope ρ1 ρ. eapply all2_same_scope; eauto.
+    have S2: same_scope ρ2 ρ. eapply all2_same_scope; eauto. 
+    have SS: same_scope ρ1 ρ2. 
+    { transitivity ρ; auto. symmetry; auto. }
+    eexists. eapply join_finite_env; eauto.
     repeat split.
-    eapply join_finite_env; eauto.
-    eapply join_lub; eauto.
-    intros d dm.
+    + eapply join_lub; eauto.
+    + intros d dm.
     inversion dm; subst.
-    eapply me. eapply join_sub_right. eauto. 
-    eapply me. eapply join_sub_left. eauto.
+    eapply me. eapply join_sub_right; eauto. auto. 
+    eapply me. eapply join_sub_left; eauto. auto.
 Qed.
 
 Lemma APPLY_continuous {D E ρ}{NE : nonempty_env ρ}{w} :
@@ -346,7 +449,7 @@ Lemma APPLY_continuous {D E ρ}{NE : nonempty_env ρ}{w} :
     -> monotone_env D 
     -> monotone_env E
     -> exists ρ3 , 
-      finite_env ρ3 /\ ρ3 ⊆e  ρ 
+      exists (pf : finite_env ρ3) , ρ3 ⊆e  ρ 
       /\ (w ∈ ((D ρ3) ▩ (E ρ3))).
 Proof.  
   intros [V [VwDp [VEp VN]]].
@@ -357,6 +460,9 @@ Proof.
     (continuous_In_sub E ρ NE mE V VEp)
       as [ ρ2 [ fρ2 [ ρ2ρ VEp2 ]]].
   intros v vV. eapply IHE; eauto.
+  have S1: same_scope ρ1 ρ. eapply all2_same_scope; eauto.
+  have S2: same_scope ρ2 ρ. eapply all2_same_scope; eauto.
+  have SS: same_scope ρ1 ρ2. { transitivity ρ; auto. symmetry; auto. }
   exists (ρ1 ⊔e ρ2).
   repeat split.
   - eapply join_finite_env; eauto.
@@ -364,11 +470,11 @@ Proof.
   - exists V. 
     have VwDp3 : V ↦ w ∈ D (ρ1 ⊔e ρ2).
     { eapply mD. 2: eapply VwDp1. 
-      intros x v z. left.  auto. }
+      eapply join_sub_left. auto. }
     have VEρ3 : mem V ⊆ E (ρ1 ⊔e ρ2).
     { intros v vV. eapply mE.
       2: eapply VEp2; auto. 
-      intros x m z. right. auto. }
+      eapply join_sub_right.  auto. }
     repeat split.
     + auto.
     + auto.
@@ -377,64 +483,618 @@ Qed.
 
 
 Lemma env_tail {ρ' x v ρ} :  
-  ρ' ⊆e (x ⤇ v ● ρ) -> finite_env ρ' -> 
+  ρ' ⊆e (x ~ v ++ ρ) -> finite_env ρ' -> 
   nonempty_env ρ ->
-  exists w, exists ρ'', ρ' = (x ⤇ w ● ρ'') /\
+  exists w, exists ρ'', ρ' = (x ~ w ++ ρ'') /\
                 (w ⊆ v) /\
-                ρ'' ⊆e ρ /\
-                finite_env ρ''.
+                exists (pf : finite_env ρ''), 
+                ρ'' ⊆e ρ.                
 Proof.
   intros h k ne.
-  move: (ne x) => [ vv I ].
-  exists (ρ' x). exists (x ⤇ ⌈ vv ⌉ ● ρ'). 
-  repeat split.
-  + extensionality y.
-    unfold env_cons. destruct (x == y). subst. auto. auto.
-  + move: (h x) => ll. unfold env_cons in ll. 
-    rewrite eq_dec_refl in ll. auto.
-  + intros y. move: (h y) => ll.
-    unfold env_cons in *.
-    destruct (x == y). subst.  
-    cbv. intros x hh. inversion hh. subst. auto. auto.
-  + unfold finite_env in *.
-    intros y.
-      unfold env_cons.
-      destruct (x == y). subst.
-      exists (cons vv nil). split. cbv.
-      split. intros x h0. inversion h0. auto.
-      intros x h0. destruct h0. subst. reflexivity. done.
-      done.
-      destruct (k y) as [E [F G]].
-      exists E. split; auto.
+  inversion h. subst.
+  exists a1.  exists E1.
+  repeat split; auto. inversion k.  auto.
 Qed.
 
 Lemma Lambda_continuous {E ρ} {NE : nonempty_env ρ}{ v x} :
-  v ∈ Λ (fun D => E (x ⤇ D ● ρ)) 
+  v ∈ Λ (fun D => E (x ~ D ++ ρ)) 
   -> (forall V, V <> nil -> 
-          continuous_env E (x ⤇ mem V ● ρ))
+          continuous_env E (x ~ mem V ++ ρ))
   -> monotone_env E
-  -> exists ρ', finite_env ρ' /\
+  -> exists ρ', exists (pf:finite_env ρ'),
             ρ' ⊆e ρ /\
-            (v ∈ (Λ (fun D => E (x ⤇ D ● ρ')))).
+            (v ∈ (Λ (fun D => E (x ~ D ++ ρ')))).
 Proof.
   induction v.
   - intro h. inversion h.
   - intros [ wEVρ VN ] IH mE.
     destruct (IH l VN v wEVρ) as
       [ ρ' [ fρ' [ ρ'Vρ wEρ' ]]]. 
-    edestruct (env_tail ρ'Vρ fρ' NE) as 
-      [ w [ ρ'' [ EQ [ WV [ S T]]]]].
-    exists ρ''. subst.
-    repeat split.
-    + auto.
-    + auto.
-    + eapply mE; eauto. 
-      intros y.
-      unfold env_cons.
-      destruct (x == y); auto. reflexivity.
-    + done.
+    inversion ρ'Vρ. subst. clear ρ'Vρ.
+    inversion fρ'. subst. clear fρ'.
+    exists E1. exists X.
+    repeat split; eauto.
+    eapply mE. 2: exact wEρ'.
+    have SS: E1 ⊆e E1. eapply Reflexive_sub_env.  eapply all2_uniq1; eauto. 
+    auto.
   - exists (initial_finite_env ρ NE).
-    repeat split.
-    eapply (initial_fin ρ NE).
-    eapply (initial_fin_sub ρ NE).
+    repeat split; eauto.
 Qed.
+
+(* -------------------------- *)
+
+(* https://github.com/jsiek/denotational_semantics/blob/master/agda/ISWIMPValue.agda *)
+
+Import LCNotations.
+Open Scope tm.
+
+(* The precondition for asking for a denotation of a term with some environment
+   is that the term should be well-scoped by that environment.
+   The advantage of locally nameless representation is that we are agnostic
+   to the order of free variables. However, environments and contexts naturally 
+   have such an order.
+ *)
+
+
+Inductive scoped t (ρ : Env) :=
+  scoped_intro : fv_tm t [<=] dom ρ -> uniq ρ -> lc_tm t -> scoped t ρ.
+
+#[global] Hint Constructors scoped : core.
+
+
+(* Find a new variable that isn't in the domain of the environment. *)
+Definition fresh_for (VS : atoms) := fresh (AtomSetImpl.elements VS).
+Lemma fresh_for_fresh : forall x VS, x = fresh_for VS -> x `notin` VS.
+Proof.
+  intros. unfold fresh_for in H.
+  move: (Atom.fresh_not_in (AtomSetImpl.elements VS)) => Frx0.
+  rewrite <- H in Frx0.
+  intro h.
+  apply AtomSetImpl.elements_1 in h.
+  eapply InA_In in h.
+  done.
+Qed.
+
+#[local] Hint Rewrite size_tm_open_tm_wrt_tm_var : lngen.
+
+(* Denotation function: unbound variables have no denotation. *)
+Fixpoint denot_n (n : nat) (a : tm) (ρ : Env) : P Value :=
+  match n with
+  | O => fun _ => False
+  | S m => 
+     match a with 
+     | var_b _ => fun _ => False 
+     | var_f x => ρ ⋅ x 
+     | app t u   => 
+         denot_n m t ρ ▩ denot_n m u ρ
+     | abs t => 
+         let x := fresh_for (dom ρ \u fv_tm t) in 
+         Λ (fun D => denot_n m (t ^ x) (x ~ D ++ ρ))
+     end
+  end.
+
+Lemma size_is_enough : forall n a, n >= size_tm a -> forall ρ, denot_n n a ρ = denot_n (size_tm a) a ρ.
+Proof.
+  intros n.
+  induction n; intros; simpl in *. 
+  + destruct a; simpl in H; lia.
+  + destruct a; simpl in *; auto.
+    - f_equal.
+      extensionality D.
+      remember (fresh_for (dom ρ \u fv_tm a)) as x.
+      rewrite IHn.
+      autorewrite with lngen. lia.
+      autorewrite with lngen. auto.
+    - 
+Admitted.
+
+
+Definition denot (a : tm) := denot_n (size_tm a) a.
+
+Lemma denot_var : forall x ρ, denot (var_f x) ρ = ρ ⋅ x.
+Proof.
+  intros. reflexivity.
+Qed.
+
+Lemma denot_app : forall t u ρ, 
+    denot (app t u) ρ = 
+      (denot t ρ ▩ denot u ρ).
+Proof. 
+  intros.
+  unfold denot. simpl.
+  rewrite size_is_enough. lia. auto.
+  rewrite size_is_enough. lia. auto.
+Qed.
+
+(* To compute the denotation of an abstraction, we need to first prove a
+   renaming lemma. This lemma ensures that the names that we pick for the
+   lambda-bound variables don't matter.  *)
+
+Ltac name_binder x0 Frx0 := 
+    match goal with 
+      [ |- context[fresh_for ?ρ] ] => 
+         remember (fresh_for ρ) as x0;
+         move: (fresh_for_fresh x0 ρ ltac:(auto)) => Frx0
+    end.
+
+Definition access_app_P := @access_app (P Value) (fun _ => False).
+
+(* Renaming property for denotations. Do we need all of these
+   scoping constraints? *)
+
+Lemma rename_denot_n : forall n t y w ρ1 ρ2 D, 
+  w `notin` dom ρ1 -> 
+  y `notin` dom ρ1 \u fv_tm t -> 
+(*   fv_tm t [<=] {{ w }} \u dom (ρ1 ++ ρ2) -> *)
+  denot_n n t (ρ1 ++ w ~ D ++ ρ2) = 
+  denot_n n (t [w ~> var_f y]) (ρ1 ++ y ~ D ++ ρ2).
+Proof. 
+  induction n;
+  intros t y w ρ1 ρ2 D Frw Fry; simpl. auto.
+  destruct t; simpl; auto.
+  all: simpl_env in Frw.
+  all: simpl_env in Fry.
+(*   all: simpl in Frt; simpl_env in Frt. *)
+  + destruct (x == w).
+    ++ subst. 
+       simpl_env.       
+       rewrite access_app_fresh; auto. rewrite access_eq_var.
+       rewrite access_app_fresh; auto. rewrite access_eq_var. auto.
+    ++ have NEx: x <> y. simpl in Fry. fsetdec.
+       edestruct (@access_app_P ρ1 x).
+       repeat rewrite H. auto.
+       destruct (H (cons (w, D) ρ2)).
+       rewrite H1. 
+       destruct (H (cons (y, D) ρ2)).
+       rewrite H3.
+       simpl. destruct (x == w) eqn:h; try done. rewrite h.
+       destruct (x == y) eqn:h1; try done. rewrite h1. auto.
+  + f_equal.
+    extensionality D0.
+    name_binder x0 Frx0.
+    name_binder y0 Fry0.
+
+    pick fresh z.
+    rewrite (subst_tm_intro z _ (var_f x0)). 
+    auto. 
+    rewrite (subst_tm_intro z _ (var_f y0)). 
+    autorewrite with lngen. auto. 
+    replace (t [w ~> var_f y] ^ z) with ((t ^ z) [w ~> var_f y]).
+    2: {
+      rewrite subst_tm_open_tm_wrt_tm; auto.
+      rewrite subst_neq_var. 
+      fsetdec.
+      auto.
+    } 
+    rewrite <- cons_app_assoc.
+
+    replace (((x0, D0) :: ρ1) ++ (w, D) :: ρ2) with
+      (nil ++ (x0 ~ D0) ++ (ρ1 ++ (w ~ D) ++ ρ2)). 2: { simpl_env; auto. }
+    rewrite <- IHn; simpl_env; auto.
+    2: { rewrite fv_tm_open_tm_wrt_tm_upper. simpl. 
+         clear Fry0 Frw Fry.
+         simpl_env in Frx0.
+         fsetdec.
+    }
+
+    replace ((y0 ~ D0) ++ ρ1 ++ (y ~ D) ++ ρ2) with
+      (nil ++ (y0 ~ D0) ++ (ρ1 ++ (y ~ D) ++ ρ2)). 2: { simpl_env; auto. }
+
+    rewrite <- IHn; simpl_env; auto.
+    2: { rewrite fv_tm_subst_tm_upper.
+         rewrite fv_tm_open_tm_wrt_tm_upper. simpl. 
+         clear Frx0 Frw Fry.
+         simpl_env in Fry0. 
+         rewrite <- fv_tm_subst_tm_lower in Fry0.
+         fsetdec.
+    }
+    
+    repeat rewrite <- (app_assoc _ (z ~ D0)).
+    eapply IHn.
+    simpl_env. auto.
+    rewrite fv_tm_open_tm_wrt_tm_upper.
+    simpl_env. simpl.
+
+    clear Frx0 Fry0 Frw.
+    simpl in Fry.
+    fsetdec.
+  + simpl_env.
+    f_equal.
+    apply IHn; simpl_env; auto.
+    simpl in Fry. fsetdec.
+    apply IHn; simpl_env; auto.
+    simpl in Fry. fsetdec.
+Qed.
+
+
+Lemma rename_open_denot : forall w y n t  ρ D, 
+  w `notin` fv_tm t -> 
+  y `notin` fv_tm t -> 
+  denot_n n (t ^ w) (w ~ D ++ ρ) = 
+  denot_n n (t ^ y) (y ~ D ++ ρ).
+Proof. 
+  intros.
+  pick fresh z.
+  rewrite (subst_tm_intro z _ (var_f w)). auto.
+  rewrite (subst_tm_intro z _ (var_f y)). auto.
+  rewrite_env (nil ++ w ~ D ++ ρ).
+  rewrite <- rename_denot_n; simpl; auto.
+  rewrite_env (nil ++ y ~ D ++ ρ).
+  rewrite <- rename_denot_n; simpl; auto.
+  rewrite fv_tm_open_tm_wrt_tm_upper. simpl. fsetdec.
+  rewrite fv_tm_open_tm_wrt_tm_upper. simpl. fsetdec.
+Qed.  
+
+
+Lemma denot_abs : forall x t ρ,
+    x `notin` dom ρ \u fv_tm t ->
+    denot (abs t) ρ = 
+      Λ (fun D => denot (t ^ x) (x ~ D ++ ρ)).
+Proof.
+  intros.
+  unfold denot. simpl.
+  rewrite size_tm_open_tm_wrt_tm_var.
+  f_equal.
+  extensionality D.
+  name_binder x0 Frx0.
+  simpl_env. 
+  rewrite -> (rename_open_denot x0 x); eauto.
+Qed.
+
+
+Lemma weaken_denot_n : forall n t ρ ρ1 ρ2, 
+    fv_tm t [<=] dom (ρ1 ++ ρ2) ->
+    uniq (ρ1 ++ ρ ++ ρ2) ->
+    denot_n n t (ρ1 ++ ρ2) = denot_n n t (ρ1 ++ ρ ++ ρ2). 
+Proof.
+  induction n.
+  all: intros t ρ ρ1 ρ2 St U.
+  all: destruct t; simpl_env in St; simpl in St; simpl; auto.
+  + (* var case *)
+    destruct_uniq.
+    move: (access_app_P ρ1 x) => [A1|A2].
+    rewrite A1. rewrite A1. auto.
+    move: (A2 ρ2) => [A21 A22].
+    rewrite A22.
+    move: (A2 (ρ ++ ρ2)) => [A31 A32].
+    rewrite A32.
+    rewrite access_app_fresh; auto.
+    intro h.
+    solve_uniq.
+  + (* abs case *)
+    f_equal.
+    extensionality D.
+    name_binder x0 Frx0.
+    name_binder y0 Fry0.
+    pick fresh z.
+    rewrite (rename_open_denot x0 z); auto.
+    rewrite (rename_open_denot y0 z); auto.
+    rewrite <- app_assoc.
+    erewrite IHn. simpl_env; eauto.
+    rewrite fv_tm_open_tm_wrt_tm_upper. simpl_env. simpl.
+    clear Frx0. clear Fry0. clear Fr. fsetdec.
+    solve_uniq.
+  + (* app case *)
+    f_equal.
+    eapply IHn; simpl_env; eauto.
+    fsetdec.
+    eapply IHn; simpl_env; eauto.
+    fsetdec.
+Qed.
+
+Lemma weaken_denot : forall t ρ2 ρ,
+   fv_tm t [<=] dom ρ2 ->
+   uniq (ρ ++ ρ2) ->
+   denot t ρ2 = denot t (ρ ++ ρ2). 
+Proof.
+  intros.
+  unfold denot.
+  eapply weaken_denot_n with (ρ1 := nil); simpl; auto.
+Qed.
+
+Lemma subst_denot_n : forall n, forall t x u ρ1 ρ2, 
+    size_tm t <= n ->
+    scoped t (ρ1 ++ x ~ (denot u ρ2) ++ ρ2) ->
+    scoped u ρ2 ->
+    denot_n n t (ρ1 ++ x ~ (denot u ρ2) ++ ρ2) =
+    denot (t [ x ~> u]) (ρ1 ++ ρ2).
+Proof.
+  induction n.
+  intros. destruct t; simpl in H; lia.
+  intros t x u ρ1 ρ2 SZ ST SU.
+  destruct t; simpl in *. 
+  all: move: ST => [FV U LC]; simpl in FV; simpl_env in FV.
+  all: move: SU => [FVu Uu LCu].    
+  all: destruct_uniq.
+  all: inversion LC; clear LC.
+  + destruct (x0 == x) eqn:EQ. subst. 
+    rewrite access_app_fresh; auto.
+    rewrite access_eq_var. 
+    apply weaken_denot; auto.
+    rewrite denot_var.
+    destruct (access_app_P ρ1 x0) as [h1 | h2].
+    rewrite h1. rewrite h1. auto.
+    move: (h2 ρ2) => [N1 N2]. rewrite N2.
+    move: (h2 (x ~ denot u ρ2 ++ ρ2)) => [N3 N4]. rewrite N4.
+    simpl. destruct (x0 == x) eqn:h. done. rewrite h. done.
+  + name_binder x0 Frx0.  simpl_env in Frx0.
+    pick fresh z. (* must be fresh for u too. *)
+    rewrite (denot_abs z). 
+    simpl_env. rewrite fv_tm_subst_tm_upper. fsetdec. 
+
+    f_equal.
+    extensionality D. 
+    simpl_env.
+
+    rewrite (rename_open_denot x0 z); simpl; simpl_env; auto.
+
+    replace (t [x ~> u] ^ z) with ((t ^ z)[x ~> u]). 
+    2: { 
+      rewrite subst_tm_open_tm_wrt_tm; auto. 
+      rewrite subst_neq_var. fsetdec. auto. 
+    }
+
+    rewrite <- app_assoc.
+    rewrite IHn; eauto.
+    autorewrite with lngen; lia.
+
+    econstructor.
+    rewrite fv_tm_open_tm_wrt_tm_upper. simpl_env. simpl. clear Fr. fsetdec.
+    solve_uniq. auto.
+  + unfold denot. simpl.
+    f_equal.
+    rewrite IHn; eauto. lia.
+    econstructor; simpl_env; auto. fsetdec. 
+    rewrite size_is_enough. lia. reflexivity.
+    rewrite IHn; eauto. lia. 
+    econstructor; simpl_env; auto. fsetdec. 
+    rewrite size_is_enough. lia. reflexivity.
+Qed.
+
+
+Lemma subst_denot : forall t x u ρ2, 
+    scoped t (x ~ (denot u ρ2) ++ ρ2) ->
+    scoped u ρ2 ->
+    denot t (x ~ (denot u ρ2) ++ ρ2) =
+    denot (t [ x ~> u]) ρ2.
+Proof.
+  intros.
+  unfold denot.
+  eapply subst_denot_n with (ρ1 := nil); eauto.
+Qed.
+
+(* ------------------------------------ *)
+
+(* denotational_semantics/agda/SemanticProperties.agda  *)
+
+Lemma denot_monotone {ρ ρ' t} : 
+  scoped t ρ ->
+  scoped t ρ' ->
+  ρ ⊆e ρ' ->
+  denot t ρ ⊆ denot t ρ'.
+Proof.
+  intros.
+  unfold denot.
+  remember (size_tm t) as n. clear Heqn.
+  move: ρ ρ' t H H0 H1.
+  induction n.
+  all: intros ρ ρ' t [FV1 U1 LC1] [FV2 U2 _] S; simpl; auto.
+  reflexivity.
+  all: destruct t; inversion LC1; simpl in FV1 ; simpl in FV2.
+  + (* var case *)
+    subst.
+    eapply all2_access; eauto.
+  + intro x.
+    unfold In , Λ.
+    destruct x; try done.
+    name_binder y Fry.
+    name_binder z Frz.
+    pick fresh w.
+    simpl_env.
+    rewrite -> (rename_open_denot y w); auto.
+    rewrite -> (rename_open_denot z w); auto.
+    intros [h1 h2].
+    split; auto.
+    specialize (IHn (w ~ mem l ++ ρ) (w ~ mem l ++  ρ')). 
+    eapply IHn; eauto.
+    repeat split; eauto.
+    rewrite fv_tm_open_tm_wrt_tm_upper; simpl. fsetdec.
+    repeat split; eauto.
+    rewrite fv_tm_open_tm_wrt_tm_upper; simpl. fsetdec.
+    eapply extend_sub_env; eauto.
+  + subst.
+    eapply APPLY_mono_sub.
+    eapply IHn; eauto. econstructor; eauto. fsetdec. econstructor; eauto. fsetdec.
+    eapply IHn; eauto. econstructor; eauto. fsetdec. econstructor; eauto. fsetdec.
+Qed.
+
+
+(* ⟦⟧-monotone-one *)
+Lemma denot_monotone_one : forall ρ t x, 
+    (forall D, scoped t (x ~ D ++ ρ))
+    -> monotone (fun D => denot t (x ~ D ++ ρ)).
+Proof. 
+  intros.
+  unfold monotone. 
+  intros D1 D2 sub.
+  move: (H D1) => [FV U1 _]. destruct_uniq. simpl_env in FV.
+  eapply denot_monotone; simpl; auto.
+  eapply H. eapply H.
+  econstructor; eauto.
+Qed.
+  
+(* ⟦⟧-continuous *)
+Lemma denot_continuous {n t ρ} :
+  n >= size_tm t
+  -> scoped t ρ 
+  -> nonempty_env ρ
+  -> continuous_env (denot_n n t) ρ.
+Proof.
+  move: t ρ.
+  induction n.
+  all: intros t ρ SZ [FV U LC] NE.
+  all: cbn.
+  all: unfold continuous_env. 
+  all: intros v.
+  all: unfold continuous_In. 
+  all: intros vIn.
+  all: try done.
+  destruct t; simpl in FV.
+  done.
+  + exists (single_env x ⌈ v ⌉ ρ NE).
+    exists (@single_fin v x ρ NE).
+    split.
+    ++ eapply single_sub. auto.
+    ++ eapply v_single_xvx. fsetdec.
+  + move: vIn. name_binder y Fry.
+    simpl in SZ. 
+    move=> vIn.
+    move: (@Lambda_continuous _ _ NE v y vIn) => h.
+    destruct h as [ρ' [F' [S' vv]]].
+    ++ intros V NV. 
+       eapply IHn. rewrite size_tm_open_tm_wrt_tm_var; try lia.
+       admit.
+       move: (nonnil_nonempty_mem NV) => h. 
+       eapply extend_nonempty_env; auto.
+       admit.
+    ++ unfold monotone_env.
+       intros.
+       rewrite size_is_enough. admit.
+       rewrite size_is_enough. admit.
+       eapply denot_monotone.
+       admit. (* The definition of monotone doesn't include a scoping 
+                 constraint, and the envs are abstract, so this isn't 
+                 satisfiable. Need to fix. *)
+       admit.
+       auto.
+    ++ exists ρ'. exists F'.
+       repeat split. auto.
+       name_binder z Frz.
+       admit. (* rename bound variable *)
+  + 
+Admitted.
+
+(*
+Lambda_continuous:
+  forall {E : list (atom * P Value) -> P Value} {ρ : Env},
+  nonempty_env ρ ->
+  forall (v : Value) (x : atom),
+  v ∈ Λ (fun D : P Value => E (x ~ D ++ ρ)) ->
+  (forall V : list Value, V <> nil -> continuous_env E (x ~ mem V ++ ρ)) ->
+  monotone_env E -> exists (ρ' : Env) (_ : finite_env ρ'), ρ' ⊆e ρ /\ (v ∈ Λ (fun D : P Value => E (x ~ D ++ ρ'))) *)
+
+
+(* ⟦⟧-continuous-⊆ *) 
+Lemma denot_continuous_sub {ρ t} : 
+  scoped t ρ
+  -> nonempty_env ρ
+  -> forall V, mem V ⊆ denot t ρ
+  -> exists ρ', exists (pf : finite_env ρ'),
+        ρ' ⊆e ρ  /\  (mem V ⊆ denot t ρ').
+Proof.
+  intros SC NE_ρ V VinEρ.
+  eapply continuous_In_sub; eauto.
+  unfold monotone_env.
+  intros r0 r'.
+  eapply denot_monotone.
+  admit. 
+  admit.
+  intros v vInV.
+  eapply denot_continuous; auto.
+Admitted.
+
+(* ⟦⟧-continuous-one *)
+Lemma denot_continuous_one { t ρ x } :
+  scoped (abs t) ρ ->
+  nonempty_env ρ ->
+  x `notin` dom ρ ->
+  continuous (fun D => denot (t ^ x) (x ~ D ++ ρ)).
+Proof.
+  intros SC NE_ρ Fr.
+  unfold continuous.
+  intros X E E_sub_denot NE_X.
+  edestruct (@denot_continuous_sub (x ~ X ++ ρ)) as 
+    [ρ' [pf [h1 h2]]]. 3: eauto.
+  + admit.
+  + eapply extend_nonempty_env; eauto.
+Admitted.
+
+
+(* Λ⟦⟧-▪-id *)
+Lemma Λ_denot_APPLY_id :
+  forall t ρ x X,
+    nonempty X
+    -> x `notin` dom ρ 
+    -> ((Λ (fun D => denot (t ^ x) (x ~ D ++ ρ))) ▩ X) ≃
+      denot (t ^ x) (x ~ X ++ ρ).
+Proof.
+  intros.
+  move: (@Λ_APPLY_id (fun D => denot (t ^ x) (x ~ D ++ ρ)) X) => h.
+  eapply h.
+  + (* continuity *)
+Admitted.
+
+
+(* Soundness of reduction with respect to denotation *)
+(* ISWIMPValue.agda *)
+
+Inductive value : tm -> Prop :=
+  | v_abs : forall t, value (abs t)
+  | v_var : forall x, value (var_f x).
+
+Lemma value_nonempty {t}{ρ} : 
+  scoped t ρ ->
+  nonempty_env ρ -> value t -> nonempty (denot t ρ).
+Proof. 
+  intros sc NEρ vv.
+  inversion sc. clear sc.
+  inversion vv; subst; clear vv; simpl in H.
+  + pick fresh x.
+    erewrite denot_abs with (x:=x); eauto.
+    exists v_fun. cbn. auto.
+  + rewrite denot_var.
+    unfold nonempty_env in NEρ.
+    eapply (@allT_access _ (fun _ => False) _ _) in NEρ.
+    2: instantiate (1:= x); auto.
+    destruct NEρ. exists x0. auto.
+Qed.
+
+Lemma soundness: 
+  forall t u, 
+    full_reduction t u ->
+    forall ρ,
+    scoped t ρ ->
+    scoped u ρ ->
+    nonempty_env ρ ->
+    denot t ρ ≃ denot u ρ.
+Proof.
+  intros t u RED. 
+  induction RED; intros ρ SCt SCu NE.
+  - (* beta *)
+    destruct SCt as [FV U lc]. inversion lc. subst.
+    simpl in FV.
+    rewrite denot_app.
+    pick fresh x.
+    erewrite denot_abs with (x:=x).
+    rewrite Λ_denot_APPLY_id.
+    eapply value_nonempty; auto.
+    econstructor; eauto. fsetdec.
+    admit. (* value u !! *)
+    fsetdec.
+    rewrite (subst_tm_intro x t u); auto.
+    rewrite subst_denot.
+    econstructor; eauto. 
+    rewrite fv_tm_open_tm_wrt_tm_upper. simpl. fsetdec.
+    admit. (* lc *)
+    econstructor; eauto. 
+    fsetdec.
+    reflexivity.
+    fsetdec.
+  - (* abs-cong *)
+    pick fresh x.
+    repeat erewrite denot_abs with (x:=x); try fsetdec.
+    specialize (H0 x ltac:(auto)).
+    eapply Λ_ext.
+    intro X.
+    eapply H0.
+Admitted.
